pull epilogue out of kf
* create epilogue function
* hide forall+ for owned cells in gC
* make everything type check locally in batch

dist/Kuiper_BasicFloat.cu
@@ -3,6 +3,7 @@
 #include "Kuiper_BasicFloat.h"
 
 __global__
+
 /**
   hoisted when extracting main
 */
