dist/Kuiper_GEMM_BlockTiling2D.cu
@@ -1,0 +1,542 @@
+
+
+#include "Kuiper_GEMM_BlockTiling2D.h"
+
+__global__
+/**
+  hoisted when extracting matmul_f32_64x64x8_8x8_rrr
+*/
+static void
+__hoisted_0(
+  size_t shared,
+  size_t cols,
+  size_t mshared,
+  size_t mcols,
+  float_t *gA4,
+  float_t *gB4,
+  float_t *gC4
+)
+{
+  float_t *sA = (float_t *)KPR_SHMEM_AT((size_t)0U);
+  float_t *sB = (float_t *)KPR_SHMEM_AT((size_t)2048U);
+  size_t mrow = blockIdx.x / mcols;
+  size_t mcol = blockIdx.x % mcols;
+  float_t rAcol[8U];
+  memset(rAcol, 0U, (size_t)8U * sizeof (float_t));
+  float_t rBrow[8U];
+  memset(rBrow, 0U, (size_t)8U * sizeof (float_t));
+  float_t rchProd[64U];
+  memset(rchProd, 0U, (size_t)64U * sizeof (float_t));
+  size_t bkIdx = (size_t)0U;
+  while (bkIdx < mshared)
+  {
+    __syncthreads();
+    size_t __anf200179 = bkIdx;
+    size_t i = threadIdx.x;
+    while (i < (size_t)512U)
+    {
+      sA[i / (size_t)8U * (size_t)8U + i % (size_t)8U] =
+        gA4[(mrow * (size_t)64U + i / (size_t)8U) * shared +
+          __anf200179 * (size_t)8U + i % (size_t)8U];
+      i += (size_t)64U;
+    }
+    size_t i1 = threadIdx.x;
+    while (i1 < (size_t)512U)
+    {
+      sB[i1 / (size_t)64U * (size_t)64U + i1 % (size_t)64U] =
+        gB4[(__anf200179 * (size_t)8U + i1 / (size_t)64U) * cols +
+          mcol * (size_t)64U + i1 % (size_t)64U];
+      i1 += (size_t)64U;
+    }
+    __syncthreads();
+    size_t dotIdx = (size_t)0U;
+    while (dotIdx < (size_t)8U)
+    {
+      size_t i0 = (size_t)0U;
+      while (i0 < (size_t)8U)
+      {
+        rAcol[i0] = sA[(threadIdx.x / (size_t)8U * (size_t)8U + i0) * (size_t)8U + dotIdx];
+        i0 += (size_t)1U;
+      }
+      size_t i1 = (size_t)0U;
+      while (i1 < (size_t)8U)
+      {
+        rBrow[i1] = sB[dotIdx * (size_t)64U + threadIdx.x % (size_t)8U * (size_t)8U + i1];
+        i1 += (size_t)1U;
+      }
+      size_t resIdxM = (size_t)0U;
+      while (resIdxM < (size_t)8U)
+      {
+        size_t resIdxN = (size_t)0U;
+        while (resIdxN < (size_t)8U)
+        {
+          rchProd[resIdxM * (size_t)8U + resIdxN] += rAcol[resIdxM] * rBrow[resIdxN];
+          resIdxN += (size_t)1U;
+        }
+        resIdxM += (size_t)1U;
+      }
+      dotIdx += (size_t)1U;
+    }
+    bkIdx += (size_t)1U;
+  }
+  size_t mrow1 = blockIdx.x / mcols;
+  size_t mcol1 = blockIdx.x % mcols;
+  size_t resIdxM = (size_t)0U;
+  while (resIdxM < (size_t)8U)
+  {
+    size_t resIdxN = (size_t)0U;
+    while (resIdxN < (size_t)8U)
+    {
+      gC4[(mrow1 * (size_t)64U + threadIdx.x / (size_t)8U * (size_t)8U + resIdxM) * cols +
+        mcol1 * (size_t)64U + threadIdx.x % (size_t)8U * (size_t)8U + resIdxN]
+      = rchProd[resIdxM * (size_t)8U + resIdxN];
+      resIdxN += (size_t)1U;
+    }
+    resIdxM += (size_t)1U;
+  }
+}
+
+float_t
+*Kuiper_GEMM_BlockTiling2D_matmul_f32_64x64x8_8x8_rrr(
+  size_t rows,
+  size_t shared,
+  size_t cols,
+  float_t *a,
+  float_t *b
+)
+{
+  float_t *gA = (float_t *)KPR_GPU_ALLOC((size_t)4U, rows * shared);
+  float_t *gB = (float_t *)KPR_GPU_ALLOC((size_t)4U, shared * cols);
+  float_t *gC = (float_t *)KPR_GPU_ALLOC((size_t)4U, rows * cols);
+  MUST(cudaMemcpy(gA, a, (size_t)4U * (rows * shared), cudaMemcpyHostToDevice));
+  MUST(cudaMemcpy(gB, b, (size_t)4U * (shared * cols), cudaMemcpyHostToDevice));
+  KPR_GUARD(rows % (size_t)64U == (size_t)0U);
+  KPR_GUARD(shared % (size_t)8U == (size_t)0U);
+  KPR_GUARD(cols % (size_t)64U == (size_t)0U);
+  size_t mcols = cols / (size_t)64U;
+  KPR_KCALL(__hoisted_0,
+    rows / (size_t)64U * mcols,
+    (size_t)64U,
+    (size_t)4096U,
+    shared,
+    cols,
+    shared / (size_t)8U,
+    mcols,
+    gA,
+    gB,
+    gC);
+  cudaDeviceSynchronize();
+  KRML_CHECK_SIZE(sizeof (float_t), rows * cols);
+  float_t *c = (float_t *)KRML_HOST_MALLOC(sizeof (float_t) * (rows * cols));
+  if (c != NULL)
+    memset(c, 0U, rows * cols * sizeof (float_t));
+  MUST(cudaMemcpy(c, gC, (size_t)4U * (rows * cols), cudaMemcpyDeviceToHost));
+  MUST(cudaFree(gA));
+  MUST(cudaFree(gB));
+  MUST(cudaFree(gC));
+  return c;
+}
+
+__global__
+/**
+  hoisted when extracting matmul_f32_32x32x32_32x8_rrr
+*/
+static void
+__hoisted_1(
+  size_t shared,
+  size_t cols,
+  size_t mshared,
+  size_t mcols,
+  float_t *gA4,
+  float_t *gB4,
+  float_t *gC4
+)
+{
+  float_t *sA = (float_t *)KPR_SHMEM_AT((size_t)0U);
+  float_t *sB = (float_t *)KPR_SHMEM_AT((size_t)4096U);
+  size_t mrow = blockIdx.x / mcols;
+  size_t mcol = blockIdx.x % mcols;
+  float_t rAcol[32U];
+  memset(rAcol, 0U, (size_t)32U * sizeof (float_t));
+  float_t rBrow[8U];
+  memset(rBrow, 0U, (size_t)8U * sizeof (float_t));
+  float_t rchProd[256U];
+  memset(rchProd, 0U, (size_t)256U * sizeof (float_t));
+  size_t bkIdx = (size_t)0U;
+  while (bkIdx < mshared)
+  {
+    __syncthreads();
+    size_t __anf200179 = bkIdx;
+    size_t i = threadIdx.x;
+    while (i < (size_t)1024U)
+    {
+      sA[i / (size_t)32U * (size_t)32U + i % (size_t)32U] =
+        gA4[(mrow * (size_t)32U + i / (size_t)32U) * shared +
+          __anf200179 * (size_t)32U + i % (size_t)32U];
+      i += (size_t)4U;
+    }
+    size_t i1 = threadIdx.x;
+    while (i1 < (size_t)1024U)
+    {
+      sB[i1 / (size_t)32U * (size_t)32U + i1 % (size_t)32U] =
+        gB4[(__anf200179 * (size_t)32U + i1 / (size_t)32U) * cols +
+          mcol * (size_t)32U + i1 % (size_t)32U];
+      i1 += (size_t)4U;
+    }
+    __syncthreads();
+    size_t dotIdx = (size_t)0U;
+    while (dotIdx < (size_t)32U)
+    {
+      size_t i0 = (size_t)0U;
+      while (i0 < (size_t)32U)
+      {
+        rAcol[i0] = sA[(threadIdx.x / (size_t)4U * (size_t)32U + i0) * (size_t)32U + dotIdx];
+        i0 += (size_t)1U;
+      }
+      size_t i1 = (size_t)0U;
+      while (i1 < (size_t)8U)
+      {
+        rBrow[i1] = sB[dotIdx * (size_t)32U + threadIdx.x % (size_t)4U * (size_t)8U + i1];
+        i1 += (size_t)1U;
+      }
+      size_t resIdxM = (size_t)0U;
+      while (resIdxM < (size_t)32U)
+      {
+        size_t resIdxN = (size_t)0U;
+        while (resIdxN < (size_t)8U)
+        {
+          rchProd[resIdxM * (size_t)8U + resIdxN] += rAcol[resIdxM] * rBrow[resIdxN];
+          resIdxN += (size_t)1U;
+        }
+        resIdxM += (size_t)1U;
+      }
+      dotIdx += (size_t)1U;
+    }
+    bkIdx += (size_t)1U;
+  }
+  size_t mrow1 = blockIdx.x / mcols;
+  size_t mcol1 = blockIdx.x % mcols;
+  size_t resIdxM = (size_t)0U;
+  while (resIdxM < (size_t)32U)
+  {
+    size_t resIdxN = (size_t)0U;
+    while (resIdxN < (size_t)8U)
+    {
+      gC4[(mrow1 * (size_t)32U + threadIdx.x / (size_t)4U * (size_t)32U + resIdxM) * cols +
+        mcol1 * (size_t)32U + threadIdx.x % (size_t)4U * (size_t)8U + resIdxN]
+      = rchProd[resIdxM * (size_t)8U + resIdxN];
+      resIdxN += (size_t)1U;
+    }
+    resIdxM += (size_t)1U;
+  }
+}
+
+float_t
+*Kuiper_GEMM_BlockTiling2D_matmul_f32_32x32x32_32x8_rrr(
+  size_t rows,
+  size_t shared,
+  size_t cols,
+  float_t *a,
+  float_t *b
+)
+{
+  float_t *gA = (float_t *)KPR_GPU_ALLOC((size_t)4U, rows * shared);
+  float_t *gB = (float_t *)KPR_GPU_ALLOC((size_t)4U, shared * cols);
+  float_t *gC = (float_t *)KPR_GPU_ALLOC((size_t)4U, rows * cols);
+  MUST(cudaMemcpy(gA, a, (size_t)4U * (rows * shared), cudaMemcpyHostToDevice));
+  MUST(cudaMemcpy(gB, b, (size_t)4U * (shared * cols), cudaMemcpyHostToDevice));
+  KPR_GUARD(rows % (size_t)32U == (size_t)0U);
+  KPR_GUARD(shared % (size_t)32U == (size_t)0U);
+  KPR_GUARD(cols % (size_t)32U == (size_t)0U);
+  size_t mcols = cols / (size_t)32U;
+  KPR_KCALL(__hoisted_1,
+    rows / (size_t)32U * mcols,
+    (size_t)4U,
+    (size_t)8192U,
+    shared,
+    cols,
+    shared / (size_t)32U,
+    mcols,
+    gA,
+    gB,
+    gC);
+  cudaDeviceSynchronize();
+  KRML_CHECK_SIZE(sizeof (float_t), rows * cols);
+  float_t *c = (float_t *)KRML_HOST_MALLOC(sizeof (float_t) * (rows * cols));
+  if (c != NULL)
+    memset(c, 0U, rows * cols * sizeof (float_t));
+  MUST(cudaMemcpy(c, gC, (size_t)4U * (rows * cols), cudaMemcpyDeviceToHost));
+  MUST(cudaFree(gA));
+  MUST(cudaFree(gB));
+  MUST(cudaFree(gC));
+  return c;
+}
+
+__global__
+/**
+  hoisted when extracting g_gemm_f32_64x64x8_8x8_rrr
+*/
+static void
+__hoisted_2(
+  float_t alpha,
+  float_t beta,
+  size_t shared,
+  size_t cols,
+  size_t mshared,
+  size_t mcols,
+  float_t *gA4,
+  float_t *gB4,
+  float_t *gC4
+)
+{
+  float_t *sA = (float_t *)KPR_SHMEM_AT((size_t)0U);
+  float_t *sB = (float_t *)KPR_SHMEM_AT((size_t)2048U);
+  size_t mrow = blockIdx.x / mcols;
+  size_t mcol = blockIdx.x % mcols;
+  float_t rAcol[8U];
+  memset(rAcol, 0U, (size_t)8U * sizeof (float_t));
+  float_t rBrow[8U];
+  memset(rBrow, 0U, (size_t)8U * sizeof (float_t));
+  float_t rchProd[64U];
+  memset(rchProd, 0U, (size_t)64U * sizeof (float_t));
+  size_t bkIdx = (size_t)0U;
+  while (bkIdx < mshared)
+  {
+    __syncthreads();
+    size_t __anf200179 = bkIdx;
+    size_t i = threadIdx.x;
+    while (i < (size_t)512U)
+    {
+      sA[i / (size_t)8U * (size_t)8U + i % (size_t)8U] =
+        gA4[(mrow * (size_t)64U + i / (size_t)8U) * shared +
+          __anf200179 * (size_t)8U + i % (size_t)8U];
+      i += (size_t)64U;
+    }
+    size_t i1 = threadIdx.x;
+    while (i1 < (size_t)512U)
+    {
+      sB[i1 / (size_t)64U * (size_t)64U + i1 % (size_t)64U] =
+        gB4[(__anf200179 * (size_t)8U + i1 / (size_t)64U) * cols +
+          mcol * (size_t)64U + i1 % (size_t)64U];
+      i1 += (size_t)64U;
+    }
+    __syncthreads();
+    size_t dotIdx = (size_t)0U;
+    while (dotIdx < (size_t)8U)
+    {
+      size_t i0 = (size_t)0U;
+      while (i0 < (size_t)8U)
+      {
+        rAcol[i0] = sA[(threadIdx.x / (size_t)8U * (size_t)8U + i0) * (size_t)8U + dotIdx];
+        i0 += (size_t)1U;
+      }
+      size_t i1 = (size_t)0U;
+      while (i1 < (size_t)8U)
+      {
+        rBrow[i1] = sB[dotIdx * (size_t)64U + threadIdx.x % (size_t)8U * (size_t)8U + i1];
+        i1 += (size_t)1U;
+      }
+      size_t resIdxM = (size_t)0U;
+      while (resIdxM < (size_t)8U)
+      {
+        size_t resIdxN = (size_t)0U;
+        while (resIdxN < (size_t)8U)
+        {
+          rchProd[resIdxM * (size_t)8U + resIdxN] += rAcol[resIdxM] * rBrow[resIdxN];
+          resIdxN += (size_t)1U;
+        }
+        resIdxM += (size_t)1U;
+      }
+      dotIdx += (size_t)1U;
+    }
+    bkIdx += (size_t)1U;
+  }
+  size_t mrow1 = blockIdx.x / mcols;
+  size_t mcol1 = blockIdx.x % mcols;
+  size_t resIdxM = (size_t)0U;
+  while (resIdxM < (size_t)8U)
+  {
+    size_t resIdxN = (size_t)0U;
+    while (resIdxN < (size_t)8U)
+    {
+      size_t vresIdxM = resIdxM;
+      size_t vresIdxN = resIdxN;
+      gC4[(mrow1 * (size_t)64U + threadIdx.x / (size_t)8U * (size_t)8U + vresIdxM) * cols +
+        mcol1 * (size_t)64U + threadIdx.x % (size_t)8U * (size_t)8U + vresIdxN]
+      =
+        beta *
+          gC4[(mrow1 * (size_t)64U + threadIdx.x / (size_t)8U * (size_t)8U + vresIdxM) * cols +
+            mcol1 * (size_t)64U + threadIdx.x % (size_t)8U * (size_t)8U + vresIdxN]
+        + alpha * rchProd[resIdxM * (size_t)8U + resIdxN];
+      resIdxN += (size_t)1U;
+    }
+    resIdxM += (size_t)1U;
+  }
+}
+
+void
+Kuiper_GEMM_BlockTiling2D_g_gemm_f32_64x64x8_8x8_rrr(
+  float_t alpha,
+  float_t beta,
+  size_t rows,
+  size_t shared,
+  size_t cols,
+  float_t *gA,
+  float_t *gB,
+  float_t *gC
+)
+{
+  KPR_GUARD(rows % (size_t)64U == (size_t)0U);
+  KPR_GUARD(shared % (size_t)8U == (size_t)0U);
+  KPR_GUARD(cols % (size_t)64U == (size_t)0U);
+  size_t mcols = cols / (size_t)64U;
+  KPR_KCALL(__hoisted_2,
+    rows / (size_t)64U * mcols,
+    (size_t)64U,
+    (size_t)4096U,
+    alpha,
+    beta,
+    shared,
+    cols,
+    shared / (size_t)8U,
+    mcols,
+    gA,
+    gB,
+    gC);
+  cudaDeviceSynchronize();
+}
+
+__global__
+/**
+  hoisted when extracting g_gemm_f32_128x128x8_8x8_rrr
+*/
+static void
+__hoisted_3(
+  float_t alpha,
+  float_t beta,
+  size_t shared,
+  size_t cols,
+  size_t mshared,
+  size_t mcols,
+  float_t *gA4,
+  float_t *gB4,
+  float_t *gC4
+)
+{
+  float_t *sA = (float_t *)KPR_SHMEM_AT((size_t)0U);
+  float_t *sB = (float_t *)KPR_SHMEM_AT((size_t)4096U);
+  size_t mrow = blockIdx.x / mcols;
+  size_t mcol = blockIdx.x % mcols;
+  float_t rAcol[8U];
+  memset(rAcol, 0U, (size_t)8U * sizeof (float_t));
+  float_t rBrow[8U];
+  memset(rBrow, 0U, (size_t)8U * sizeof (float_t));
+  float_t rchProd[64U];
+  memset(rchProd, 0U, (size_t)64U * sizeof (float_t));
+  size_t bkIdx = (size_t)0U;
+  while (bkIdx < mshared)
+  {
+    __syncthreads();
+    size_t __anf200179 = bkIdx;
+    size_t i = threadIdx.x;
+    while (i < (size_t)1024U)
+    {
+      sA[i / (size_t)8U * (size_t)8U + i % (size_t)8U] =
+        gA4[(mrow * (size_t)128U + i / (size_t)8U) * shared +
+          __anf200179 * (size_t)8U + i % (size_t)8U];
+      i += (size_t)256U;
+    }
+    size_t i1 = threadIdx.x;
+    while (i1 < (size_t)1024U)
+    {
+      sB[i1 / (size_t)128U * (size_t)128U + i1 % (size_t)128U] =
+        gB4[(__anf200179 * (size_t)8U + i1 / (size_t)128U) * cols +
+          mcol * (size_t)128U + i1 % (size_t)128U];
+      i1 += (size_t)256U;
+    }
+    __syncthreads();
+    size_t dotIdx = (size_t)0U;
+    while (dotIdx < (size_t)8U)
+    {
+      size_t i0 = (size_t)0U;
+      while (i0 < (size_t)8U)
+      {
+        rAcol[i0] = sA[(threadIdx.x / (size_t)16U * (size_t)8U + i0) * (size_t)8U + dotIdx];
+        i0 += (size_t)1U;
+      }
+      size_t i1 = (size_t)0U;
+      while (i1 < (size_t)8U)
+      {
+        rBrow[i1] = sB[dotIdx * (size_t)128U + threadIdx.x % (size_t)16U * (size_t)8U + i1];
+        i1 += (size_t)1U;
+      }
+      size_t resIdxM = (size_t)0U;
+      while (resIdxM < (size_t)8U)
+      {
+        size_t resIdxN = (size_t)0U;
+        while (resIdxN < (size_t)8U)
+        {
+          rchProd[resIdxM * (size_t)8U + resIdxN] += rAcol[resIdxM] * rBrow[resIdxN];
+          resIdxN += (size_t)1U;
+        }
+        resIdxM += (size_t)1U;
+      }
+      dotIdx += (size_t)1U;
+    }
+    bkIdx += (size_t)1U;
+  }
+  size_t mrow1 = blockIdx.x / mcols;
+  size_t mcol1 = blockIdx.x % mcols;
+  size_t resIdxM = (size_t)0U;
+  while (resIdxM < (size_t)8U)
+  {
+    size_t resIdxN = (size_t)0U;
+    while (resIdxN < (size_t)8U)
+    {
+      size_t vresIdxM = resIdxM;
+      size_t vresIdxN = resIdxN;
+      gC4[(mrow1 * (size_t)128U + threadIdx.x / (size_t)16U * (size_t)8U + vresIdxM) * cols +
+        mcol1 * (size_t)128U + threadIdx.x % (size_t)16U * (size_t)8U + vresIdxN]
+      =
+        beta *
+          gC4[(mrow1 * (size_t)128U + threadIdx.x / (size_t)16U * (size_t)8U + vresIdxM) * cols +
+            mcol1 * (size_t)128U + threadIdx.x % (size_t)16U * (size_t)8U + vresIdxN]
+        + alpha * rchProd[resIdxM * (size_t)8U + resIdxN];
+      resIdxN += (size_t)1U;
+    }
+    resIdxM += (size_t)1U;
+  }
+}
+
+void
+Kuiper_GEMM_BlockTiling2D_g_gemm_f32_128x128x8_8x8_rrr(
+  float_t alpha,
+  float_t beta,
+  size_t rows,
+  size_t shared,
+  size_t cols,
+  float_t *gA,
+  float_t *gB,
+  float_t *gC
+)
+{
+  KPR_GUARD(rows % (size_t)128U == (size_t)0U);
+  KPR_GUARD(shared % (size_t)8U == (size_t)0U);
+  KPR_GUARD(cols % (size_t)128U == (size_t)0U);
+  size_t mcols = cols / (size_t)128U;
+  KPR_KCALL(__hoisted_3,
+    rows / (size_t)128U * mcols,
+    (size_t)256U,
+    (size_t)8192U,
+    alpha,
+    beta,
+    shared,
+    cols,
+    shared / (size_t)8U,
+    mcols,
+    gA,
+    gB,
+    gC);
+  cudaDeviceSynchronize();
+}
+
