dist/Kuiper_GEMM_BlockTiling2D.h
@@ -1,0 +1,52 @@
+
+
+#ifndef __Kuiper_GEMM_BlockTiling2D_H
+#define __Kuiper_GEMM_BlockTiling2D_H
+
+#include <kuiper.h>
+
+float_t
+*Kuiper_GEMM_BlockTiling2D_matmul_f32_64x64x8_8x8_rrr(
+  size_t rows,
+  size_t shared,
+  size_t cols,
+  float_t *a,
+  float_t *b
+);
+
+float_t
+*Kuiper_GEMM_BlockTiling2D_matmul_f32_32x32x32_32x8_rrr(
+  size_t rows,
+  size_t shared,
+  size_t cols,
+  float_t *a,
+  float_t *b
+);
+
+void
+Kuiper_GEMM_BlockTiling2D_g_gemm_f32_64x64x8_8x8_rrr(
+  float_t alpha,
+  float_t beta,
+  size_t rows,
+  size_t shared,
+  size_t cols,
+  float_t *gA,
+  float_t *gB,
+  float_t *gC
+);
+
+void
+Kuiper_GEMM_BlockTiling2D_g_gemm_f32_128x128x8_8x8_rrr(
+  float_t alpha,
+  float_t beta,
+  size_t rows,
+  size_t shared,
+  size_t cols,
+  float_t *gA,
+  float_t *gB,
+  float_t *gC
+);
+
+
+#define __Kuiper_GEMM_BlockTiling2D_H_DEFINED
+#endif
