dist/Kuiper_HReduce.cu
@@ -3,6 +3,7 @@
 #include "Kuiper_HReduce.h"
 
 __global__
+
 /**
   hoisted when extracting reduce_f16_plus
 */
@@ -13,14 +14,14 @@ static void __hoisted_0(size_t lena, half_t *a)
   {
     size_t __anf14641 = n;
     __syncthreads();
-    size_t nextid = threadIdx.x + (size_t)(1U << (uint32_t)__anf14641);
+    size_t nextid = threadIdx_x + (size_t)(1U << (uint32_t)__anf14641);
     if (nextid < lena)
       if
       (
-        (threadIdx.x & (size_t)(1U << (uint32_t)(__anf14641 + (size_t)1U)) - (size_t)1U) ==
+        (threadIdx_x & (size_t)(1U << (uint32_t)(__anf14641 + (size_t)1U)) - (size_t)1U) ==
           (size_t)0U
       )
-        a[threadIdx.x] = __hadd(a[threadIdx.x], a[nextid]);
+        a[threadIdx_x] = __hadd(a[threadIdx_x], a[nextid]);
     n += (size_t)1U;
   }
 }
@@ -32,6 +33,7 @@ void Kuiper_HReduce_reduce_f16_plus(size_t lena, half_t *a)
 }
 
 __global__
+
 /**
   hoisted when extracting reduce_f32_plus
 */
@@ -42,14 +44,14 @@ static void __hoisted_1(size_t lena, float_t *a)
   {
     size_t __anf14641 = n;
     __syncthreads();
-    size_t nextid = threadIdx.x + (size_t)(1U << (uint32_t)__anf14641);
+    size_t nextid = threadIdx_x + (size_t)(1U << (uint32_t)__anf14641);
     if (nextid < lena)
       if
       (
-        (threadIdx.x & (size_t)(1U << (uint32_t)(__anf14641 + (size_t)1U)) - (size_t)1U) ==
+        (threadIdx_x & (size_t)(1U << (uint32_t)(__anf14641 + (size_t)1U)) - (size_t)1U) ==
           (size_t)0U
       )
-        a[threadIdx.x] += a[nextid];
+        a[threadIdx_x] += a[nextid];
     n += (size_t)1U;
   }
 }
@@ -61,6 +63,7 @@ void Kuiper_HReduce_reduce_f32_plus(size_t lena, float_t *a)
 }
 
 __global__
+
 /**
   hoisted when extracting reduce_f64_plus
 */
@@ -71,14 +74,14 @@ static void __hoisted_2(size_t lena, double_t *a)
   {
     size_t __anf14641 = n;
     __syncthreads();
-    size_t nextid = threadIdx.x + (size_t)(1U << (uint32_t)__anf14641);
+    size_t nextid = threadIdx_x + (size_t)(1U << (uint32_t)__anf14641);
     if (nextid < lena)
       if
       (
-        (threadIdx.x & (size_t)(1U << (uint32_t)(__anf14641 + (size_t)1U)) - (size_t)1U) ==
+        (threadIdx_x & (size_t)(1U << (uint32_t)(__anf14641 + (size_t)1U)) - (size_t)1U) ==
           (size_t)0U
       )
-        a[threadIdx.x] += a[nextid];
+        a[threadIdx_x] += a[nextid];
     n += (size_t)1U;
   }
 }
@@ -90,6 +93,7 @@ void Kuiper_HReduce_reduce_f64_plus(size_t lena, double_t *a)
 }
 
 __global__
+
 /**
   hoisted when extracting reduce_u32_plus
 */
@@ -100,14 +104,14 @@ static void __hoisted_3(size_t lena, uint32_t *a)
   {
     size_t __anf14641 = n;
     __syncthreads();
-    size_t nextid = threadIdx.x + (size_t)(1U << (uint32_t)__anf14641);
+    size_t nextid = threadIdx_x + (size_t)(1U << (uint32_t)__anf14641);
     if (nextid < lena)
       if
       (
-        (threadIdx.x & (size_t)(1U << (uint32_t)(__anf14641 + (size_t)1U)) - (size_t)1U) ==
+        (threadIdx_x & (size_t)(1U << (uint32_t)(__anf14641 + (size_t)1U)) - (size_t)1U) ==
           (size_t)0U
       )
-        a[threadIdx.x] += a[nextid];
+        a[threadIdx_x] += a[nextid];
     n += (size_t)1U;
   }
 }
@@ -119,6 +123,7 @@ void Kuiper_HReduce_reduce_u32_plus(size_t lena, uint32_t *a)
 }
 
 __global__
+
 /**
   hoisted when extracting reduce_u64_plus
 */
@@ -129,14 +134,14 @@ static void __hoisted_4(size_t lena, uint64_t *a)
   {
     size_t __anf14641 = n;
     __syncthreads();
-    size_t nextid = threadIdx.x + (size_t)(1U << (uint32_t)__anf14641);
+    size_t nextid = threadIdx_x + (size_t)(1U << (uint32_t)__anf14641);
     if (nextid < lena)
       if
       (
-        (threadIdx.x & (size_t)(1U << (uint32_t)(__anf14641 + (size_t)1U)) - (size_t)1U) ==
+        (threadIdx_x & (size_t)(1U << (uint32_t)(__anf14641 + (size_t)1U)) - (size_t)1U) ==
           (size_t)0U
       )
-        a[threadIdx.x] += a[nextid];
+        a[threadIdx_x] += a[nextid];
     n += (size_t)1U;
   }
 }
